    $$\begin{aligned}
    e^{x}&=\sum_{n=0}^{\infty} \frac{1}{n !} x^{n}=1+x+\frac{1}{2 !} x^{2}+\cdots \in(-\infty,+\infty) \\
    \sin x&=\sum_{n=0}^{\infty} \frac{(-1)^{n}}{(2 n+1) !} x^{2 n+1}=x-\frac{1}{3 !} x^{3}+\frac{1}{5 !} x^{5}+\cdots, x \in(-\infty,+\infty) \\
    \cos x&=\sum_{n=0}^{\infty} \frac{(-1)^{n}}{(2 n) !} x^{2 n}=1-\frac{1}{2 !} x^{2}+\frac{1}{4 !} x^{4}+\cdots, x \in(-\infty,+\infty) \\
    \ln (1+x)&=\sum_{n=0}^{\infty} \frac{(-1)^{n}}{n+1} x^{n+1}=x-\frac{1}{2} x^{2}+\frac{1}{3} x^{3}+\cdots, x \in(-1,1] \\
    \frac{1}{1-x}&=\sum_{n=0}^{\infty} x^{n}=1+x+x^{2}+x^{3}+\cdots, x \in(-1,1) \\
    \frac{1}{1+x}&=\sum_{n=0}^{\infty}(-1)^{n} x^{n}=1-x+x^{2}-x^{3}+\cdots, x \in(-1,1)\\
        (1+x)^{\alpha}&=1+\sum_{n=1}^{\infty} \frac{\alpha(\alpha-1) \cdots(\alpha-n+1)}{n !} x^{n}=1+\alpha x+\frac{\alpha(\alpha-1)}{2 !} x^{2}+\cdots, x \in(-1,1) \\
        \arctan x&=\sum_{n=0}^{\infty} \frac{(-1)^{n}}{2 n+1} x^{2 n+1}=x-\frac{1}{3} x^{3}+\frac{1}{5} x^{5}+\cdots+ x \in[-1,1] \\
        \arcsin x&=\sum_{n=0}^{\infty} \frac{(2 n) !}{4^{n}(n !)^{2}(2 n+1)} x^{2n+1}=x+\frac{1}{6} x^{3}+\frac{3}{40} x^{5}+\frac{5}{112} x^{7}+\frac{35}{1152} x^{9}+\cdots+, x \in(-1,1)\\
        \tan x&=\sum_{n=1}^{\infty} \frac{B_{2 n}(-4)^{n}\left(1-4^{n}\right)}{(2 n) !} x^{2 n-1}=x+\frac{1}{3} x^{3}+\frac{2}{15} x^{5}+\frac{17}{315} x^{7}+\frac{62}{2835} x^{9}+\frac{1382}{155925} x^{11}+\frac{21844}{6081075} x^{13}+\frac{929569}{638512875} x^{15}+\cdots,x\in (-\frac{\pi}{2},\frac{\pi}{2})
    \end{aligned}$$

![[Pasted image 20241106200942.png]]
![[Pasted image 20241106201049.png]]
![[Pasted image 20241106201103.png]]

